various work

MinDepth.dfy
@@ -1,7 +1,9 @@
 
 datatype TreeNode = Nil | Cons(val: nat, left: TreeNode, right: TreeNode)
 
-predicate isPath(paths: seq<TreeNode>, root: TreeNode) {
+predicate isPath(paths: seq<TreeNode>, root: TreeNode) 
+{
+
     if |paths| == 0 then false else match paths[0] {
         case Nil => false
         case Cons(val, left, right) => if |paths| == 1 then root == paths[0] else root == paths[0] && (isPath(paths[1..], left) || isPath(paths[1..], right))
@@ -10,14 +12,14 @@ predicate isPath(paths: seq<TreeNode>, root: TreeNode) {
 
 function TreeSet(root: TreeNode): set<TreeNode> {
     match root {
-        case Nil => {Nil}
+        case Nil => {}
         case Cons(val, left, right) => TreeSet(left)+{root}+TreeSet(right)
     }
 }
 
 function ChildSet(root: TreeNode): set<TreeNode> {
     match root {
-        case Nil => {Nil}
+        case Nil => {}
         case Cons(val, left, right) => {left}+ChildSet(left)+{right}+ChildSet(right)
     }
 }
@@ -30,7 +32,11 @@ function method min(a:int,b: int): int {
     if a > b then b else a
 }
 
-function method boundedMin(a: int, b: int): int {
+function method boundedMin(a: int, b: int): int 
+    ensures a > 0 && b == 0 ==> boundedMin(a,b) == a
+    ensures a == 0 && b > 0 ==> boundedMin(a,b) == b
+    ensures a > 0 && b > 0 ==> boundedMin(a,b) == (if a < b then a else b)
+{
     if a == 0 then b else if b == 0 then a else min(a,b)
 }
 
@@ -53,7 +59,10 @@ method minDepth(root: TreeNode) returns (depth: nat)
 
     if root.left == Nil && root.right == Nil {
         assert isPath([root], root) && |[root]| == 1;
+        // allSeqsTreenode(root);
         return 1;
+        // assert depth == 1;
+        assert forall ps: seq<TreeNode> :: isPath(ps, root) ==> depth <= |ps|;
     }
     var leftDepth := minDepth(root.left);
     var rightDepth := minDepth(root.right);
@@ -61,24 +70,19 @@ method minDepth(root: TreeNode) returns (depth: nat)
         // ghost var q: seq<TreeNode> :| isPath(q, root.left) && |q| == leftDepth && forall ps: seq<TreeNode> :: isPath(ps, root.left) ==> leftDepth <= |ps|;
         ghost var q: seq<TreeNode> :| isPath(q, root.left) && |q| == leftDepth;
         assert isPath([root]+q, root) && |[root]+q| == 1 + leftDepth;
+        // assert forall ps: seq<TreeNode> :: isPath(ps, root.left) ==> isPath([root]+ps, root) && 1+leftDepth <= |[root]+ps|;
     }
     if rightDepth > 0 {
         ghost var p: seq<TreeNode> :| isPath(p, root.right) && |p| == rightDepth;
         assert isPath([root]+p, root) && |[root]+p| == 1 + rightDepth;
+        // assert forall ps: seq<TreeNode> :: isPath(ps, root.right) ==> isPath([root]+ps, root) && 1+rightDepth <= |[root]+ps|;
     }
     // if leftDepth > 0 && rightDepth > 0 {
-    //     ghost var q: seq<TreeNode> :| isPath(q, root.left) && |q| == leftDepth && forall ps: seq<TreeNode> :: isPath(ps, root.left) ==> leftDepth <= |ps|;
-    //     ghost var p: seq<TreeNode> :| isPath(p, root.right) && |p| == rightDepth && forall ps: seq<TreeNode> :: isPath(ps, root.right) ==> rightDepth <= |ps|;
-    //     ghost var ps := set px: seq<TreeNode> | isPath(px, root) ; 
-    //     if leftDepth > rightDepth {
-    //         // assert forall ps: seq<TreeNode> :: isPath([root]+q, root) ==> 1+boundedMin(leftDepth, rightDepth) <= |p|;
-
-    //     }else if rightDepth > leftDepth {
-
-    //     }else{
-
-    //     }
+    //     assert (forall pls: seq<TreeNode> :: isPath(pls, root.left) ==> leftDepth == |pls| && isPath([root]+pls, root) && 1+leftDepth <= |[root]+pls| && 1+boundedMin(leftDepth, rightDepth) <= 1+leftDepth) &&
+    //    (forall prs: seq<TreeNode> :: isPath(prs, root.right) ==> rightDepth == |prs| && isPath([root]+prs, root) && 1+rightDepth <= |[root]+prs| && 1+boundedMin(leftDepth, rightDepth) <= 1+rightDepth) ==> 
+    //    forall ps: seq<TreeNode> :: isPath(ps, root) ==> 1 + boundedMin(leftDepth, rightDepth) <= |ps|;
     // }
+
     return 1 + boundedMin(leftDepth, rightDepth);
 }
 
@@ -113,6 +117,36 @@ exists ps(ps root) && depth > |ps|
 
 
  */
+lemma allSeqsTreenode(node: TreeNode)
+    requires node != Nil && node.left == Nil && node.right == Nil
+    ensures (iset ps: seq<TreeNode> | isPath(ps, node)) == iset{[node]}
+    ensures forall ps: seq<TreeNode> :: isPath(ps, node) ==> 1 <= |ps|
+{
+    if !((iset ps: seq<TreeNode> | isPath(ps, node)) == iset{[node]}) {
+        var xs :| xs != [node] && isPath(xs, node);
+        assert xs in iset ps: seq<TreeNode> | isPath(ps, node);
+        assert |xs| > 0;
+        if xs[0] != node {
+            assert !isPath(xs, node);
+        }
+        else if |xs| > 1 && xs[0] == node && xs[1] != node {
+            assert !isPath(xs, node);
+        }
+        assert false;
+    }
+}
+
+lemma AllTreNode(node: TreeNode)
+    requires node != Nil
+    requires forall pls: seq<TreeNode> :: isPath(pls, node.left)
+    requires forall prs: seq<TreeNode> :: isPath(prs, node.left)
+    ensures forall ps: seq<TreeNode> :: isPath(ps, node)
+{
+    var xl: seq<TreeNode> :| isPath(xl, node.left);
+    var xr: seq<TreeNode> :| isPath(xr, node.right);
+    assert isPath([node]+xl, node);
+    assert isPath([node]+xr, node);
+}
 
 method Test() {
     var t := Nil;
