activitySelection.dfy
@@ -21,22 +21,60 @@ method recursiveActivitySelector(start: seq<nat>, finish: seq<nat>, k: nat, n: n
     }
 }
 
+function substructure(start: seq<nat>, finish: seq<nat>, k: nat): set<nat>
+    requires |finish| >= 1
+    requires |start| == |finish|
+    requires 0 <= k < |finish|
+    requires forall i :: 0 <= i < |finish| ==> start[i] < finish[i]
+    requires forall i,j :: 0 <= i <= j < |finish| ==> i <= j ==> finish[i] <= finish[j]
+{
+    set x | 0 <= x < |finish| && start[x] >= finish[k]
+}
+
+predicate activitySet(start: seq<nat>, finish: seq<nat>, compatible: set<nat>) 
+    requires |finish| >= 1
+    requires |start| == |finish|
+    requires forall i :: i in compatible ==> 0 < i <= |finish|
+    requires forall i :: 0 <= i < |finish| ==> start[i] < finish[i]
+    requires forall i,j :: 0 <= i <= j < |finish| ==> i <= j ==> finish[i] <= finish[j]
+{
+    forall i, j :: i in compatible && j in compatible && finish[i-1] != finish[j-1] && finish[i-1] < finish[j-1] ==> start[i-1] < start[j-1] && start[j-1] > finish[i-1]
+}
+
+method Test() {
+    /*
+    i  1 2 3 4 5 6 7 8 9 10 11 
+    si 1 3 0 5 3 5 6 8 8 2 12 
+    fi 4 5 6 7 9 9 10 11 12 14 16
+    */
+    var start :=  [1,3,0,5,3,5,6,8,8,2,12];
+    var finish := [4,5,6,7,9,9,10,11,12,14,16];
+    assert activitySet(start, finish, {1,4,8,11});
+}
+
 method activitySelector(start: seq<nat>, finish: seq<nat>) returns (A: set<nat>)
     requires |finish| >= 1
     requires |start| == |finish|
     requires forall i :: 0 <= i < |finish| ==> start[i] < finish[i]
-    requires forall i :: 0 <= i < |finish|-1 ==> finish[i] <= finish[i+1]
+    requires forall i,j :: 0 <= i <= j < |finish| ==> i <= j ==> finish[i] <= finish[j]
     ensures forall x :: x in A ==> 1 <= x <= |finish|
-    ensures forall x,y :: x in A && y in A && x < y ==> finish[x-1] < start[y-1]
+    // ensures forall x,y :: x in A && y in A && x < y ==> finish[x-1] < start[y-1]
+    ensures activitySet(start, finish, A);
 {
     var n := |finish|;
     A := {1};
     var k := 1;
     var m := 2;
     while m <= n 
-        invariant k < m
+        invariant k < m <= n+1
+        invariant 2 <= m <= n+1
+        invariant forall x :: x in A ==> 1 <= x <= |finish| && finish[k-1] >= finish[x-1]
+        invariant activitySet(start, finish, A);
     {
         if start[m-1] >= finish[k-1] {
+            assert 2 <= m <= n;
+            assert forall x :: x in A ==> 1 <= x <= |finish| && finish[k-1] >= finish[x-1] ==> forall x :: x in A ==> start[m-1] >= finish[x];
+            // assert activitySet(start, finish, A+{m});
             A := A + {m};
             k := m;
         }
