MaxContigSubarray.dfy
@@ -1,0 +1,401 @@
+
+function method max(a: int, b: int): int 
+    ensures max(a,b) == if a > b then a else b
+{
+    if a > b then a else b
+}
+
+function method sumSeq(nums: seq<int>): int 
+    ensures |nums| == 0 ==> sumSeq(nums) == 0
+    ensures |nums| > 0 ==> sumSeq(nums) == nums[0] + sumSeq(nums[1..])
+{
+    if |nums| == 0 then 0 else nums[0] + sumSeq(nums[1..])
+}
+
+function method sumSeqTail(nums: seq<int>): int 
+    ensures |nums| == 0 ==> sumSeqTail(nums) == 0
+    ensures |nums| > 0 ==> sumSeqTail(nums) == sumSeqTail(nums[..(|nums|-1)]) + nums[|nums|-1]
+{
+    if |nums| == 0 then 0 else sumSeqTail(nums[..(|nums|-1)]) + nums[|nums| - 1]
+}
+
+function reverseSeq(nums: seq<int>): seq<int>
+    ensures |reverseSeq(nums)| == |nums|
+    ensures forall i :: 0 <= i < |nums| ==> reverseSeq(nums)[i] == nums[|nums|-i-1]
+{
+ if |nums| == 0 then [] else [nums[|nums|-1]] + reverseSeq(nums[..(|nums|-1)])
+}
+
+lemma doubleReverse(nums: seq<int>) 
+    ensures reverseSeq(reverseSeq(nums)) == nums
+{
+
+}
+
+lemma splitReverse(nums: seq<int>)
+    requires |nums| > 0
+    ensures nums[1..] == reverseSeq(reverseSeq(nums)[..(|nums|-1)])
+{
+}
+
+// lemma revSeq(nums: seq<int>)
+//     ensures sumSeq(nums) == sumSeq(reverseSeq(nums))
+// {
+
+// }
+
+lemma multisetSequence(nums: seq<int>, ms: multiset<int>) 
+    requires |nums| > 0
+    requires multiset(nums[1..]) == ms;
+    ensures multiset(nums) == ms + multiset{nums[0]}
+{
+    assert nums == [nums[0]]+nums[1..];
+    var z := nums[0];
+    assert z in multiset(nums);
+    assert forall i :: 1 <= i < |nums| ==> nums[i] in ms;
+    assert forall i :: 1 <= i < |nums| ==> nums[i] in multiset(nums);
+    assert forall i :: 1 <= i < |nums| && nums[i] != nums[0] ==> multiset(nums)[nums[i]] == ms[nums[i]];
+    // if nums[0] in ms {
+    //     assert multiset(nums)[nums[0]] == ms[nums[0]]+1;
+    // }else{
+    //     assert ms[nums[0]] == 0;
+    //     assert multiset(nums)[nums[0]] == 1;
+    // }
+}
+
+lemma multisetSequenceRemove(nums: seq<int>, ms: multiset<int>) 
+    requires |nums| > 0
+    requires multiset(nums) == ms;
+    ensures multiset(nums[1..]) == ms - multiset{nums[0]}
+{
+    assert nums == [nums[0]]+nums[1..];
+}
+
+lemma multisetSequenceSplitRemove(nums: seq<int>, ms: multiset<int>, z: int, i : int) 
+    requires |nums| > 0
+    requires 0 <= i < |nums|
+    requires nums[i] == z;
+    requires multiset(nums) == ms;
+    ensures multiset(nums[..i]+nums[(i+1)..]) == ms - multiset{z}
+{
+    assert nums == nums[..i] + [z] + nums[(i+1)..];
+}
+
+lemma seqZ(nums: seq<int>, z: int)
+    requires z in nums;
+{
+    assert exists i :: 0 <= i < |nums| ==> nums[i]  == z;
+}
+
+// lemma sumSeqSplit(nums: seq<int>, z: int, i: int)
+//     requires |nums| > 0
+//     requires 0 <= i < |nums|
+//     requires nums[i] == z;
+//     ensures sumSeq(nums[..i]+nums[(i+1)..]) == sumSeq(nums) - z;
+// {
+//     assert nums == nums[..i] + [z] + nums[(i+1)..];
+//     calc {
+//         sumSeq(nums);
+//         ==
+//         sumSeq(nums[..i]+[z]+nums[(i+1)..]);
+
+//     }
+// }
+
+// lemma so(numsa: seq<int>, numsb: seq<int>)
+//     requires |numsa| == |numsb|
+//     requires multiset(numsa) == multiset(numsb)
+//     ensures sumSeq(numsa) == sumSeq(numsb)
+// {
+//     if |numsa| > 0 {
+//         assert |numsa| > 0;
+//         var z := numsa[0];
+//         assert multiset(numsa)[z] >= 1;
+//         var bz := numsa[1..];
+//         var q := multiset(numsa);
+//         var j := multiset(bz);
+//         multisetSequenceRemove(numsa, q);
+//         assert j == q - multiset{z};
+//         assert z in multiset(numsa);
+//         assert z in multiset(numsb);
+//         assert z in numsa;
+//         assert z in numsb;
+//         assert multiset(numsa) != multiset{};
+//         assert multiset(numsb) != multiset{};
+//         assert multiset(numsa[1..]) == multiset(numsa)-multiset{z};
+//         var i :| 0 <= i < |numsb| && numsb[i] == z;
+        
+//         assert numsb == numsb[..i] + [z]+ numsb[(i+1)..];
+//         var bmz := numsb[..i] + numsb[(i+1)..];
+//         multisetSequenceSplitRemove(numsb, multiset(numsb), z, i);
+//         assert j == multiset(bmz);
+//         so(bz, bmz);
+//         assert sumSeq(bz) == sumSeq(bmz);
+//         assert sumSeq(numsa) == z + sumSeq(bz);
+//         assert sumSeq(numsb) == z + sumSeq(bmz);
+//         // assert sumSeq(numsb) ==
+//         //ghost var x :| x in multiset(numsa);
+//     }
+// }
+
+// lemma someThing(nums: seq<int>) 
+//     requires |nums| >= 1
+//     ensures sumSeq(nums[1..]) == sumSeq(reverseSeq(nums)[..|nums|-1])
+// {
+
+// }
+
+// lemma reverseSum(nums: seq<int>)
+//     ensures sumSeq(nums) == sumSeq(reverseSeq(nums))
+// {
+//     if |nums| == 0 {
+
+//     } else if |nums| == 1 {
+
+//     }else {
+//         var rev := reverseSeq(nums);
+//         var k := nums[0];
+//         assert rev[|nums|-1] == k;
+        
+//         // assert sumSeqTail(reverseSeq(nums)) == k + sumSeqTail(rev[..(|nums|-1)]);
+//         assert nums[1..] == reverseSeq(rev[..(|nums|-1)]);
+//         assert sumSeq(nums) == k + sumSeq(nums[1..]);
+//         calc {
+//             sumSeq(reverseSeq(nums));
+//             ==
+//             k + sumSeq(rev[..(|nums|-1)]);
+//             == 
+//             k + sumSeq(nums[1..]);
+//             ==
+//             sumSeq(nums);
+//         }
+//     }
+// }
+
+// lemma sumSeqsEqual(nums: seq<int>) 
+//     ensures sumSeq(nums) == sumSeqTail(nums);
+// {
+//     if |nums| == 0 {
+//         assert sumSeq(nums) == 0 == sumSeqTail(nums);
+//     }else if |nums| == 1 {
+//         assert sumSeq(nums) == nums[0] == sumSeqTail(nums);
+//     }else if |nums| > 1 {
+//         var somenums := nums[1..];
+//     }
+// }
+
+method Test() {
+    var goober := [2997, 3, 3];
+    var what := multiset(goober);
+    assert what[3] > 1;
+    var goober2 := [2997,  3];
+    assert multiset(goober2) == what - multiset{3};
+    assert sumSeq(goober[0..0]) == 0;
+    assert sumSeq(goober[0..1]) == 2997;
+    assert sumSeq(goober[0..2]) == 3000;
+}
+
+// method maxContigSubarrayNaive(nums: seq<int>) returns (maxsum: int)
+//     requires |nums| >= 1
+//     ensures forall i, j :: 0 <= i <= j <= |nums| ==> maxsum >= sumSeq(nums[i..j])
+// {
+//     var n := |nums|;
+//     var maxSum := nums[0];
+//     for left := 0 to n-1 
+//         invariant 0 <= left <= n-1
+//     {
+//         for right := left to n-1 
+//             invariant left <= right <= n-1;
+//         {
+//             var windowSum := 0;
+//             ghost var wsum := sumSeq(nums[left..left]);
+//             assert wsum == 0;
+
+//             var k := left;
+//             while k <= right
+//                 invariant left <= right
+//                 invariant left <= k <= right+1
+//                 invariant windowSum == sumSeq(nums[left..k])
+//             {
+//                 windowSum := windowSum + nums[k];
+//                 k := k + 1;
+//                 wsum := sumSeq(nums[left..k]);
+//             }
+
+//             maxSum := max(maxSum, windowSum);
+//         }
+//     }
+
+
+//     return maxSum;
+// }
+
+method maxContigSubarrayBetter(nums: seq<int>) returns (maxsum: int)
+    requires |nums| >= 1
+{
+    var n := |nums|;
+    var maxSubarraySum := 0;
+    for left := 0 to n-1 {
+        var runningWindowSum := 0;
+        for right := left to n-1 {
+            runningWindowSum := runningWindowSum + nums[right];
+            maxSubarraySum := max(maxSubarraySum, runningWindowSum);
+        }
+    }
+    return maxSubarraySum;
+}
+
+method maxContigousSubarraySum(nums: seq<int>) returns (maxsum: int)
+    requires |nums| > 1
+{
+    var maxSoFar := nums[0];
+    var maxEndingHere :=  nums[0];
+    for i := 1 to |nums|-1 {
+        maxEndingHere := max(maxEndingHere + nums[i], nums[i]);
+        maxSoFar := max(maxSoFar, maxEndingHere);
+    }
+    return maxSoFar;
+}
+
+// method simpleSum(row: seq<int>, left: int, right: int) returns (sum: int) 
+//     requires 0 <= left <= right < |row|
+//     ensures sum == sumSeq(row[left..(right+1)])
+// {
+//     sum := 0;
+//     var k := left; 
+//     while k <= right 
+//         invariant left <= k <= right+1
+//         invariant sum == sumSeq(row[left..k])
+//     {
+//         sum := sum + row[k];
+//         k := k + 1;
+//     }
+//     assert k == right+1;
+
+// }
+
+// lemma sumSeqSplit(a: seq<int>, i: int)
+//     requires 0 <= i <= |a|
+//     ensures sumSeq(a) == sumSeq(a[..i]) + sumSeq(a[i..])
+// {
+//     assert a == a[..i] + a[i..];
+//     if a == [] {
+//         assert a[..0] == [];
+//         assert a[0..] == [];
+//         assert sumSeq(a) == 0;
+//     } else if i == |a| && a[i..] == [] {
+//         assert a == a[..i] + [];
+//         assert a == a[..i];
+//         // assert sumSeq(a[i..]) == 0;
+//         calc {
+//             sumSeq(a);
+//             == 
+//             sumSeq(a[..i]) + sumSeq(a[i..]);
+//             ==
+//             sumSeq(a)+sumSeq([]);
+//             ==
+//             sumSeq(a)+0;
+//             ==
+//             sumSeq(a);
+//         }
+//     }else if a[..i] != [] {
+//         var p := sumSeq(a[..i]);
+//         var s := sumSeq(a[i..]);
+//         assert a[..i] == a[..(i-1)] +[a[i-1]];
+//         assert a[(i-1)..] == [a[i-1]]+a[i..];
+//         assert s + a[i-1] == sumSeq(a[(i-1)..]);
+//         sumSeqSplit(a[..(i-1)],i-1);
+//         assert sumSeq(a[..(i-1)]) == sumSeq(a[..(i-1)]) + sumSeq([a[i-1]]);
+
+//     }
+// }
+
+// lemma sumSeqConcat(a: seq<int>, b: seq<int>)
+//     ensures sumSeq(a+b) == sumSeq(a) + sumSeq(b)
+// {
+//     if a == [] {
+//         assert sumSeq(a) + sumSeq(b) == sumSeq(a+b);
+//     }else if b == [] {
+//         assert sumSeq(a) + sumSeq(b) == sumSeq(a+b);
+//     }else if |a| == 1 {
+//         assert sumSeq(a) == a[0];
+//         assert sumSeq(a+b) == a[0] + sumSeq(b);
+//     }else{
+//         calc {
+//             sumSeq(a+b);
+//             == 
+//             sumSeq(a[..(|a|-1)]+[a[|a|-1]]+ b);
+//             == 
+//             sumSeq(a[..(|a|-1)]) + sumSeq([a[|a|-1]]+ b);
+//         }
+//     }
+// }
+
+
+// lemma sumSeqCommut(row: seq<int>, k: int)
+//     requires |row| >= 1
+//     requires row[|row|-1] == k
+//     ensures sumSeq(row[..|row|-1]) == sumSeq(row)-k
+// {
+//    assert row == row[..|row|-1]+[k];
+// }
+
+lemma somethings(nums: seq<int>, sum: int, k: int)
+    requires sum == sumSeq(nums)
+    ensures sumSeq([sum,k]) == sumSeq([k]+nums)
+{
+
+}
+
+//    ([1,2,3]+[4]) == 10 == (1+(2+(3+(4))))
+//    ([4]+[1,2,3]) == 10 == (4+(1+(2+(3))))
+// lemma sumSeqCommut(row: seq<int>, k: int)
+//     ensures sumSeq(row+[k]) == sumSeq([k]+row)
+// {
+//     if row == [] {
+//         assert sumSeq([]+[k]) == sumSeq([k]+[]);
+//     }else if |row| == 1 {
+//         assert row == [row[0]];
+//         // assert sumSeq([row[0]]+[k]) == sumSeq([k]+[row[0]]);
+//         calc {
+//             sumSeq(row+[k]);
+//             ==
+//             sumSeq([row[0]]+[k]);
+//             ==
+//             row[0]+sumSeq([k]);
+//             ==
+//             row[0]+k;
+//             ==
+//             k+row[0];
+//             ==
+//             k+sumSeq([row[0]]);
+//             ==
+//             sumSeq([k]+[row[0]]);
+//             ==
+//             sumSeq([k]+row);
+//         }
+
+//     }else if |row| == 2 {
+//         assert row == [row[0],row[1]];
+
+//     }else{
+
+//     }
+//     // var oldSum := sumSeq(row);
+//     // assert oldSum + k == sumSeq([k]+row);
+//     // assert oldSum + k == sumSeq(row+[k]);
+
+// }
+
+lemma sumSeqs(row: seq<int>, left: int, k: int)
+    requires 0 <= left <= k < |row|-1
+    // ensures sumSeq(row[left..k+1]) == sumSeq(row[left..k]) + row[k]
+{
+    assert row[left..k+1] == row[left..k]+[row[k]];
+    calc {
+        sumSeq(row[left..k+1]);
+        ==
+        sumSeq(row[left..k]+[row[k]]);
+    }
+
+}
