lambdaCalc.dfy
@@ -1,0 +1,72 @@
+datatype Nat = Zero | Succ(Pred: Nat)
+
+function add(m: Nat, n: Nat) : Nat
+decreases m
+{
+    match m
+    case Zero => n
+    case Succ(m') => Succ(add(m', n))
+}
+
+function multiply(m: Nat, n: Nat): Nat
+  decreases m
+{
+  match m
+    case Zero => Zero
+    case Succ(Zero) => n
+    case Succ(p) => add(n, multiply(p, n))
+}
+
+lemma CommAdd(m: Nat, n: Nat)
+ensures add(m,n) == add(n, m)
+{
+    match m
+    case Zero => Add1(n);
+    case Succ(m') => CommAdd(m', n);
+}
+
+lemma Multiply1(m: Nat)
+decreases m
+// ensures multiply(m, Zero) == Zero
+ensures multiply(m, Succ(Zero)) == m
+{
+//
+}
+// a(b + c) = ab + ac;
+lemma distributiveLaw(a: Nat, b: Nat, c: Nat)
+    ensures multiply(a, add(b,c)) == add(multiply(a,b), multiply(a,c))
+{
+    if b == Zero {
+
+    }
+
+}
+/*
+   m * n 
+== S m' * n
+== n + m' * n
+{ using CommMulti property}
+== n + n * m'
+{ using distributive property }
+== n * (1 + m')
+== n * m
+*/
+// lemma CommMult(m: Nat, n: Nat)
+//   ensures multiply(m, n) == multiply(n, m)
+// {
+//   match m
+//     case Zero => {}
+//     case Succ(Zero) => Multiply1(n);
+//     case Succ(m') => {
+//       calc {
+//         multiply(Succ(m'), n);
+//         // defintion of multiply
+//         add(n, multiply(m', n));
+//         { CommMult(m', n); }
+//         add(n, multiply(n, m'));
+//         { Multiply1(n); }
+//         add(multiply(n, Succ(Zero)), multiply(n, m'));
+//         // TODO use distributive law
+//       }
+//     }
+// }
