matrixAdd.dfy
@@ -1,0 +1,19 @@
+
+
+method matrixAdd(left: array2<real>, right: array2<real>, m: nat, n: nat) returns (result: array2<real>)
+    requires m > 0 && n > 0
+    requires left.Length0 == right.Length0 && left.Length0 == m && left.Length1 == right.Length1 && left.Length1 == n
+    ensures result.Length0 == left.Length0 && result.Length1 == left.Length1
+    ensures forall i, j :: 0 <= i < m && 0 <= j < n ==> result[i,j] == left[i,j] + right[i,j]
+{
+    result := new real[m,n];
+    for i := 0 to m -1 
+        invariant forall x, j :: x < i && 0 <= j < n ==> result[x,j] == left[x,j] + right[x,j];
+    {
+        for j := 0 to n - 1 
+            invariant j > 0 ==> result[i,j] == left[i,j] + right[i,j];
+        {
+            result[i,j] := left[i,j] + right[i,j];
+        }
+    }
+}
